src/rpartrec.lean
@@ -4,14 +4,13 @@ import computability.partrec_code
 import computability.halting
 import data.pfun
 import tactic
-import code
 
 open encodable denumerable roption
 
 namespace nat
 
 inductive rpartrec (o : ℕ →. ℕ) : (ℕ →. ℕ) → Prop
-| oracle : rpartrec (λ x, o x)
+| oracle : rpartrec o
 | zero : rpartrec (pure 0)
 | succ : rpartrec succ
 | left : rpartrec ↑(λ n : ℕ, n.unpair.1)
@@ -21,8 +20,6 @@ inductive rpartrec (o : ℕ →. ℕ) : (ℕ →. ℕ) → Prop
 | prec {f g} : rpartrec f → rpartrec g → rpartrec (unpaired (λ a n,
     n.elim (f a) (λ y IH, do i ← IH, g (mkpair a (mkpair y i)))))
 | rfind {f} : rpartrec f → rpartrec (λ a, rfind (λ n, (λ m, m = 0) <$> f (mkpair a n)))
-| univn {f : ℕ →. ℕ} [decidable_pred f.dom] : rpartrec f → rpartrec (unpaired $ λ a n, 
-    nat.rpartrec.code.evaln a.unpair.1 f.eval_opt (of_nat _ a.unpair.2) n)
 
 namespace rpartrec
 
@@ -63,7 +60,6 @@ begin
   assume pgf phg,
   induction pgf,
   case oracle { exact phg },
-  case univn : _ _ _ pf { exactI univn pf },
   case zero { exact zero },
   case succ { exact succ },
   case left { exact left },
@@ -199,167 +195,3 @@ theorem refl_in (f : α → β) : f computable_in (f : α →. β) := nat.rpartr
   f computable_in (g : β →. τ)→ g computable_in h → f computable_in h := nat.rpartrec.trans
 
 end rcomputable
-
-namespace nat.rpartrec.code
-open nat.rpartrec (code)
---
---private lemma evaln_comp' {c f} {g : ℕ → option ℕ} (h : eval f c = (λ x, g x)) : ∀ m, ∃ s₀,
---  ∀ n a, n < m → g n = some a → evaln s₀ f c n = some a := λ m,
---begin
---  induction m with m0 ih, simp,
---  rcases ih with ⟨s₀, hs₀⟩,
---  cases e : g m0 with v,
---  { refine ⟨s₀, λ n a en ha, _⟩,
---    have : n < m0 ∨ n = m0, from nat.lt_succ_iff_lt_or_eq.mp en,
---    cases this, { exact hs₀ _ _ this ha },
---    { exfalso, rw this at ha, rw e at ha, exact option.not_mem_none a ha } },
---  { unfold_coes at h,
---    have : v ∈ eval f c m0, simp[h, e],
---    have : ∃ k, v ∈ evaln k f c m0 := evaln_complete.mp this, rcases this with ⟨s₁, hs₁⟩,
---    refine ⟨max s₀ s₁, _⟩,
---    intros n a en ha,
---    have en' : n < m0 ∨ n = m0, from nat.lt_succ_iff_lt_or_eq.mp en,
---    cases en', 
---    { have : evaln s₀ f c n = option.some a := hs₀ _ _ en' ha,
---      show evaln (max s₀ s₁) f c n = option.some a,
---        from evaln_mono (le_max_left s₀ s₁) this },
---    { rw en', 
---      have : a = v, from option.some_inj.mp (by simp only [←e, ←ha, en']),
---      show evaln (max s₀ s₁) f c m0 = option.some a, rw this,
---        from evaln_mono (le_max_right s₀ s₁) hs₁ } }
---end
---
-@[simp] lemma eval_eval_opt {α β} (f : α →. β) [D : decidable_pred f.dom] {x} :
-  f.eval_opt x = @roption.to_option _ (f x) (D x) := rfl
-
-lemma eq_none_or_eq_some_dec {α} (o : roption α) [decidable o.dom] : o = none ∨ ∃ x, o = some x :=
-by { exact eq_none_or_eq_some o }
-
-private lemma evaln_comp_dec {c f} [D : decidable_pred (eval f c).dom] : ∀ m, ∃ s₀,
-  ∀ n a, n < m → eval f c n = some a → evaln s₀ f c n = some a := λ m,
-begin
-  induction m with m0 ih, simp,
-  rcases ih with ⟨s₀, hs₀⟩,
-  have e : eval f c m0 = none ∨ ∃ v, eval f c m0 = some v := eq_none_or_eq_some (eval f c m0),
-  cases e,
-  { refine ⟨s₀, λ n a en ha, _⟩,
-    have : n < m0 ∨ n = m0, from nat.lt_succ_iff_lt_or_eq.mp en,
-    cases this, { exact hs₀ _ _ this ha },
-    { exfalso, rw this at ha, rw e at ha, exact roption.some_ne_none _ (eq.symm ha) } },
-  { rcases e with ⟨v, e⟩,
-    have : v ∈ eval f c m0, simp[e],
-    have : ∃ k, v ∈ evaln k f c m0 := evaln_complete.mp this, rcases this with ⟨s₁, hs₁⟩,
-    refine ⟨max s₀ s₁, _⟩,
-    intros n a en ha,
-    have en' : n < m0 ∨ n = m0, from nat.lt_succ_iff_lt_or_eq.mp en,
-    cases en', 
-    { have : evaln s₀ f c n = option.some a := hs₀ _ _ en' ha,
-      show evaln (max s₀ s₁) f c n = option.some a,
-        from evaln_mono (le_max_left s₀ s₁) this },
-    { rw en', 
-      have : a = v, from roption.some_inj.mp (by simp only [←e, ←ha, en']),
-      show evaln (max s₀ s₁) f c m0 = option.some a, rw this,
-        from evaln_mono (le_max_right s₀ s₁) hs₁ } }
-end
-
-@[simp] theorem mem_to_option' {α} {o : roption α} [decidable o.dom] {a : α} :
-  to_option o = some a ↔ a ∈ o := mem_to_option
-
-theorem eval_univn_eq_dec (c f) [D : decidable_pred (eval f c).dom] : 
-  eval f c.univn = nat.unpaired (λ a n, (evaln a.unpair.fst (eval f c).eval_opt (of_nat code a.unpair.snd) n)) :=
-begin
-  funext n, apply roption.ext, intros a,
-  rw eval_univn_evaln_iff, 
-  simp[evaln_univn, (>>)], split,
-  { rintros ⟨s, hs⟩, rcases hs with ⟨e, hs⟩,
-    have : ∀ x y, evaln (s+1) f c x = some y → (eval f c).eval_opt x = some y,
-    { intros x y ey, simp[eval_eval_opt], have := evaln_sound ey, exact this },    
-    have := evaln_inclusion (λ x y e, this x y) _ _ hs,
-    exact this },
-  { assume ha, 
-    have : ∃ s₀, ∀ m a, m < n.unpair.fst.unpair.fst →
-      eval f c m = option.some a → evaln s₀ f c m = option.some a :=
-    evaln_comp_dec n.unpair.1.unpair.1, rcases this with ⟨s₀, hs₀⟩,
-    refine ⟨max n s₀, le_max_left _ _, _⟩, 
-    have hs₀' : ∀ m a, m < n.unpair.fst.unpair.fst →
-      (eval f c).eval_opt m = some a → evaln (max n s₀ + 1) f c m = option.some a,
-    from λ _ _ em ha, evaln_mono (le_trans (le_max_right n _) (nat.le_succ _)) (hs₀ _ _ em (
-      by { simp at ha, simp[of_option, roption.eq_some_iff] at ha ⊢, exact ha})),
-    exact evaln_inclusion hs₀' _ _ ha } 
-end
-
---theorem eval_univn_eq {c f} {g : ℕ → option ℕ} (h : eval f c = (λ x, g x)) : 
---  eval f c.univn = nat.unpaired (λ a n, (evaln a.unpair.fst g (of_nat code a.unpair.snd) n)) :=
---begin
---  unfold_coes at h,
---  funext n, apply roption.ext, intros a,
---  rw eval_univn_evaln_iff, 
---  simp[evaln_univn, (>>)], split,
---  { rintros ⟨s, hs⟩, rcases hs with ⟨e, hs⟩,
---    have : ∀ x y, evaln (s+1) f c x = some y → g x = some y,
---    { intros x y ey, have := evaln_sound ey, simp[h] at this, exact this },    
---    have := evaln_inclusion (λ x y e, this x y) _ _ hs,
---    exact this },
---  { assume ha, 
---    have : ∃ s₀, ∀ m a, m < n.unpair.fst.unpair.fst →
---      g m = option.some a → evaln s₀ f c m = option.some a :=
---    evaln_comp' h n.unpair.1.unpair.1, rcases this with ⟨s₀, hs₀⟩,
---    refine ⟨max n s₀, le_max_left _ _, _⟩, 
---    have hs₀' : ∀ m a, m < n.unpair.fst.unpair.fst →
---      g m = option.some a → evaln (max n s₀ + 1) f c m = option.some a,
---    from λ _ _ em ha, evaln_mono (le_trans (le_max_right n _) (nat.le_succ _)) (hs₀ _ _ em ha),
---    exact evaln_inclusion hs₀' _ _ ha } 
---end
-
-theorem rfind'' {f} : nat.rpartrec f (nat.unpaired (λ a m,
-  (nat.rfind (λ n, (λ m, m = 0) <$> f (nat.mkpair a (n + m)))).map (+ m))) :=
-rpartrec.nat_iff.mp $
-begin
-  simp,
-  have c₀ : primrec (λ (x : (ℕ × ℕ) × ℕ), x.2 + x.1.2) := 
-  primrec.nat_add.comp primrec.snd (primrec.snd.comp primrec.fst),
-  have c₁ : primrec (λ (m : ((ℕ × ℕ) × ℕ) × ℕ), to_bool (m.2 = 0)) :=
-  primrec₂.comp primrec.eq primrec.snd (primrec.const 0),
-  have c₂ : (λ (x : (ℕ × ℕ) × ℕ), f (x.1.1.mkpair (x.2 + x.1.2))) partrec_in f :=
-  rpartrec.refl.comp (primrec₂.mkpair.comp (primrec.fst.comp primrec.fst) $
-    primrec.nat_add.comp primrec.snd (primrec.snd.comp primrec.fst)).to_comp.to_rpart,
-  have := (rpartrec.rfind.trans (c₂.map c₁.to_comp.to_rcomp)).map c₀.to_comp.to_rcomp,
-  simp at this,
-  exact this.comp primrec.unpair.to_comp.to_rcomp
-end
-
-theorem exists_code {f g : ℕ →. ℕ} [D : decidable_pred g.dom] :
-  nat.rpartrec g f → ∃ c, eval (g.eval_opt) c = f := λ h,
-begin
-  induction h,
-  case nat.rpartrec.oracle 
-  { exact ⟨oracle, by { simp[eval], funext n, exact of_to_option (g n) }⟩ },  
-  case nat.rpartrec.zero   { exact ⟨zero, rfl⟩ },
-  case nat.rpartrec.succ   { exact ⟨succ, rfl⟩ },
-  case nat.rpartrec.left   { exact ⟨left, rfl⟩ },
-  case nat.rpartrec.right  { exact ⟨right, rfl⟩ },
-  case nat.rpartrec.pair : f₀ f₁ pf₀ pf₁ hf₀ hf₁
-  { rcases hf₀ with ⟨e₀, rfl⟩, rcases hf₁ with ⟨e₁, rfl⟩,
-    exact ⟨pair e₀ e₁, rfl⟩ },
-  case nat.rpartrec.comp : f₀ f₁ pf₀ pf₁ hf₀ hf₁
-  { rcases hf₀ with ⟨e₀, rfl⟩, rcases hf₁ with ⟨e₁, rfl⟩,
-    exact ⟨comp e₀ e₁, rfl⟩ },
-  case nat.rpartrec.prec : f₀ f₁ pf₀ pf₁ hf₀ hf₁
-  { rcases hf₀ with ⟨e₀, rfl⟩, rcases hf₁ with ⟨e₁, rfl⟩,
-    exact ⟨prec e₀ e₁, rfl⟩ },
-  case nat.rpartrec.rfind : f₀ pf₀ hf₀
-  { rcases hf₀ with ⟨e₀, rfl⟩, 
-    refine ⟨comp (rfind' e₀) (pair nat.rpartrec.code.id zero), _⟩,
-    simp [eval, (<*>), pure, pfun.pure, roption.map_id'],  },
-  case nat.rpartrec.univn : f₀ D pf₀ hf₀
-  { rcases hf₀ with ⟨e₀, rfl⟩,
-    have := by exactI eval_univn_eq_dec e₀ g.eval_opt,
-    refine ⟨e₀.univn, this⟩ 
-    --have : eval g.eval_opt e₀ = λ x, (@pfun.eval_opt _ _ f₀ D) x,
-    --{ unfold_coes, simp, exact h },
-    --have := eval_univn_eq this,
-    --refine ⟨e₀.univn, this⟩ },
-  }
-end
-
-end nat.rpartrec.code
